
\subsubsection{Jacobian, $J\wrap*{q_{i}}$}
\begin{equation}
	\begin{split}
		J_{11} & = -(s_{i,1} (2 J_{11} = a_{1} + 2 a_{3} c_{i,23} + 2 a_{2} c_{i,2} + a_{4} c_{i,234}))/2	\\	
		J_{12} & = -c_{i,1} (a_{3} s_{i,23} + a_{2} s_{i,2} + (a_{4} s_{i,234})/2)		\\
		J_{13} & = -c_{i,1} (a_{3} s_{i,23} + (a_{4} s_{i,234})/2)		\\
		J_{14} & = -(a_{4} s_{i,234} c_{i,1})/2\\
		J_{21} & = (c_{i,1} (2 a_{1} + 2 a_{3} c_{i,23} + 2 a_{2} c_{i,2} + a_{4} c_{i,234}))/2	\\
		J_{22} & = -s_{i,1} (a_{3} s_{i,23} + a_{2} s_{i,2} + (a_{4} s_{i,234})/2)	\\
		J_{23} & = -s_{i,1} (a_{3} s_{i,23} + (a_{4} s_{i,234})/2)		\\
		J_{24} & = -(a_{4} s_{i,234} s_{i,1})/2\\
		J_{31} & = 0		\\
		J_{32} & = a_{3} c_{i,23} + a_{2} c_{i,2} + (a_{4} c_{i,234})/2		\\
		J_{33} & = a_{3} c_{i,23} + (a_{4} c_{i,234})/2	\\
		J_{34} & = (a_{4} c_{i,234})/2\\
		J_{41} & = 0		\\
		J_{42} & = s_{i,1}	\\	
		J_{43} & = s_{i,1}	\\	
		J_{44} & = s_{i,1}\\
		J_{51} & = 0		\\
		J_{52} & = -c_{i,1}	\\	
		J_{53} & = -c_{i,1}	\\	
		J_{54} & = -c_{i,1}\\
		J_{61} & = 1		\\
		J_{62} & = 0		\\
		J_{63} & = 0		\\
		J_{64} & = 0\\
	\end{split}
	\label{eq::jac}
\end{equation}